theories/AlgTactic.ec
@@ -37,7 +37,7 @@
 require import Int.
 
 (* -------------------------------------------------------------------- *)
-theory RingCore.
+theory Requires.
   type domain.
 
   op rzero : domain.
@@ -45,6 +45,11 @@ theory RingCore.
   op add   : domain -> domain -> domain.
   op opp   : domain -> domain.
   op mul   : domain -> domain -> domain.
+  op expr  : domain -> int -> domain.
+  op ofint : int -> domain.
+  op sub   : domain -> domain -> domain.
+  op inv   : domain -> domain.
+  op div   : domain -> domain -> domain.
 
   axiom nosmt oner_neq0:
     rone <> rzero.
@@ -72,27 +77,13 @@ theory RingCore.
 
   axiom nosmt mulrDl:
     forall (x y z: domain), mul x (add y z) = add (mul x y) (mul x z).
-end RingCore.
-
-(* -------------------------------------------------------------------- *)
-theory RingIntPow.
-  clone export RingCore.
-
-  op expr : domain -> int -> domain.
 
   axiom nosmt expr0:
-    forall (x : domain), expr x 0 = rzero.
+    forall (x : domain), expr x 0 = rone.
 
   axiom nosmt exprS:
     forall (x : domain) (n : int), 0 <= n =>
       expr x (n+1) = mul x (expr x n).
-end RingNatMul.
-
-(* -------------------------------------------------------------------- *)
-theory RingOfInt.
-  clone export RingCore.
-
-  op ofint : int -> domain.
 
   axiom nosmt ofint0: ofint 0 = rzero.
   axiom nosmt ofint1: ofint 1 = rone.
@@ -102,37 +93,16 @@ theory RingOfInt.
 
   axiom nosmt ofintN:
     forall (n : int), ofint (-n) = opp (ofint n).
-end RingOfInt.
-
-(* -------------------------------------------------------------------- *)
-theory RingWithSub.
-  clone export RingCore.
-
-  op sub : domain -> domain -> domain.
 
   axiom nosmt subrE:
     forall (x y : domain), sub x y = add x (opp y).
-end RingWithSub.
-
-(* -------------------------------------------------------------------- *)
-theory FieldCore.
-  clone export RingNatMul.
-
-  op inv : domain -> domain.
 
   axiom nosmt mulrV:
     forall (x : domain), x <> rzero => mul x (inv x) = rone.
 
   axiom nosmt exprN:
     forall (x : domain) (n : int), n <= 0 => expr x (-n) = inv (expr x n).
-end FieldCore.
-
-(* -------------------------------------------------------------------- *)
-theory FieldWithDiv.
-  clone export FieldCore.
-
-  op div : domain -> domain -> domain.
 
   axiom nosmt divrE:
     forall (x y : domain), div x y = mul x (inv y).
-end FieldWithDiv.
+end Requires.
